examples/sort/CompareMain01proof.v
@@ -1,0 +1,94 @@
+Require Import HoareDef CompareMain0 CompareMain1 CompareHeader SimModSemL SimModSem.
+Require Import Coqlib.
+Require Import Universe.
+Require Import Skeleton.
+Require Import PCM.
+Require Import ModSem Behavior.
+Require Import Relation_Definitions.
+
+(*** TODO: export these in Coqlib or Universe ***)
+Require Import Relation_Operators.
+Require Import RelationPairs.
+From ITree Require Import
+     Events.MapDefault.
+From ExtLib Require Import
+     Core.RelDec
+     Structures.Maps
+     Data.Map.FMapAList.
+
+Require Import HTactics Logic YPM TODOYJ.
+
+Generalizable Variables E R A B C X Y.
+
+Set Implicit Arguments.
+
+Local Open Scope nat_scope.
+
+
+
+
+Section SIMMODSEM.
+
+  Context `{Σ: GRA.t}.
+
+  Let W: Type := (Σ * Any.t) * (Σ * Any.t).
+
+  Let wf: W -> Prop :=
+    fun '(mrps_src0, mrps_tgt0) =>
+      (<<SRC: mrps_src0 = (ε, tt↑)>>) /\
+      (<<TGT: mrps_tgt0 = (ε, tt↑)>>)
+  .
+
+  Variable global_cmpspecs: list (gname * (Z -> Z -> Z)).
+  Variable GlobalStb: SkEnv.t -> list (gname * fspec).
+
+  Variable cmpspecs_incl: 
+    forall fn fd
+           (FIND: List.find (fun '(_fn, _) => dec fn _fn) cmpspecs = Some fd),
+      List.find (fun '(_fn, _) => dec fn _fn) global_cmpspecs = Some fd.
+
+  Variable globalstb_incl
+    :
+      forall skenv fn f fn'
+             (SPECS: List.find (fun '(_fn, _) => dec fn _fn) cmpspecs = Some (fn', f)),
+      exists mn,
+        (<<FIND: List.find (fun '(_fn, _) => dec fn _fn) (GlobalStb skenv) = Some (fn, compare_gen f mn)>>).
+
+  Variable cmpspecs_globalstb
+    :
+      forall skenv fn f fn'
+             (SPECS: List.find (fun '(_fn, _) => dec fn _fn) cmpspecs = Some (fn', f)),
+      exists mn,
+        (<<FIND: List.find (fun '(_fn, _) => dec fn _fn) (GlobalStb skenv) = Some (fn, compare_gen f mn)>>).
+
+  Theorem correct: ModPair.sim (Wrap1.Wrap cmpspecs GlobalStb) Wrap0.Wrap.
+  Proof.
+    econs; ss; [|admit ""].
+    i. eapply adequacy_lift.
+    econstructor 1 with (wf:=wf); et; ss.
+    econs; ss. init. unfold wrapF, ccall. harg_tac. 
+    destruct x as [[n0 n1] f]. ss. des; subst. 
+    iPure PRE. des; clarify.
+    eapply Any.upcast_inj in PRE. des; clarify.
+    rewrite Any.upcast_downcast. ss. steps. astart 1.
+    rewrite PRE1. ss. steps. rename fn into fn0. 
+    hexploit cmpspecs_globalstb; eauto. i. des.
+    eapply APC_step_clo with (fn:=fn0) (args:=[Vint n0; Vint n1]).
+    { try by
+      eapply Ord.eq_lt_lt;
+       [ symmetry; eapply OrdArith.add_from_nat
+       | eapply OrdArith.lt_from_nat; eapply Nat.lt_add_lt_sub_r;
+          eapply Nat.lt_succ_diag_r ]. }
+    { eauto. }
+    { ss. }
+    { eapply OrdArith.lt_from_nat; eapply Nat.lt_succ_diag_r. }
+    i. subst args'. 
+    hcall_tac (n0, n1) (ord_pure 0) (@URA.unit Σ) (@URA.unit Σ) (@URA.unit Σ); ss.
+    { splits; ss. eauto with ord_step. }
+    des. iPure POST. clarify. eapply Any.upcast_inj in POST. des; clarify.
+    steps. rewrite Any.upcast_downcast in _UNWRAPN. clarify. astop. 
+    force_l. eexists.
+    hret_tac (@URA.unit Σ) (@URA.unit Σ); ss.
+  Qed.
+
+End SIMMODSEM.
