examples/sort/CompareMain1.v
@@ -1,0 +1,54 @@
+Require Import Coqlib.
+Require Import ITreelib.
+Require Import Universe.
+Require Import STS.
+Require Import Behavior.
+Require Import ModSem.
+Require Import Skeleton.
+Require Import PCM.
+Require Import HoareDef.
+Require Import CompareHeader.
+Require Import Logic.
+
+Generalizable Variables E R A B C X Y Σ.
+
+Set Implicit Arguments.
+
+
+
+Section PROOF.
+
+  Context `{Σ: GRA.t}.
+
+  Variable GlobalStb: list (gname * fspec).
+
+  Section SKENV.
+
+    Definition main_spec: fspec := mk_simple "Main" (X:=unit) 
+                                             (fun _ => (
+                                                  (fun _ o => ⌜o = ord_top⌝),
+                                                  top2
+                                             )).
+
+    Definition compare_spec:    fspec := compare_gen mycmp "Main".
+
+    Definition Mainstb: list (gname * fspec) := [("main", main_spec); ("compare", compare_spec)].
+
+    Definition Mainsbtb: list (gname * fspecbody) := [("main", mk_specbody main_spec (fun _ => APC;; trigger (Choose _))); ("compare", mk_specbody compare_spec (fun _ => trigger (Choose _)))].
+
+    Definition MainSem: ModSem.t := {|
+      ModSem.fnsems := List.map (fun '(fn, body) => (fn, fun_to_tgt GlobalStb fn body)) Mainsbtb;
+      ModSem.mn := "Main";
+      ModSem.initial_mr := ε;
+      ModSem.initial_st := tt↑;
+                                   |}
+    .
+  End SKENV.
+
+  Definition Main: Mod.t := {|
+    Mod.get_modsem := fun skenv => MainSem;
+    Mod.sk := [("compare", Sk.Gfun)];
+  |}
+  .
+
+End PROOF.
