examples/sort/Wrap1.v
@@ -1,0 +1,57 @@
+Require Import Coqlib.
+Require Import ITreelib.
+Require Import Universe.
+Require Import STS.
+Require Import Behavior.
+Require Import ModSem.
+Require Import Skeleton.
+Require Import PCM.
+Require Import HoareDef.
+Require Import MutHeader.
+Require Import Logic.
+
+Generalizable Variables E R A B C X Y Σ.
+
+Set Implicit Arguments.
+
+
+
+Section PROOF.
+
+  Context `{Σ: GRA.t}.
+
+  Variable cmpspecs: list (gname * (Z -> Z -> Z)).
+  Variable GlobalStb: SkEnv.t -> list (gname * fspec).
+
+  Section SKENV.
+    Variable skenv: SkEnv.t.
+
+    Definition wrap_spec:    fspec := mk_simple "Wrap" (X:=Z*Z*(Z -> Z -> Z))
+                                                (fun '(n0, n1, f) => (
+                                                     (fun varg o => ⌜exists fn blk, varg = [Vint n0; Vint n1; Vptr blk 0]↑ /\ o = ord_pure 1 /\ skenv.(SkEnv.blk2id) blk = Some fn /\ List.find (fun '(_fn, _) => dec fn _fn) cmpspecs = Some (fn, f)⌝), 
+                                                     (fun vret => ⌜vret = (Vint (f n0 n1))↑⌝)
+                                                )).
+
+    Definition Wrapstb: list (gname * fspec) := [("wrap", wrap_spec)].
+
+    Definition Wrapsbtb: list (gname * fspecbody) := [("wrap", mk_specbody wrap_spec (fun _ => trigger (Choose _)))].
+
+    Definition WrapSem: ModSem.t := {|
+      ModSem.fnsems := List.map (fun '(fn, body) => (fn, fun_to_tgt (GlobalStb skenv) fn body)) Wrapsbtb;
+      ModSem.mn := "Wrap";
+      ModSem.initial_mr := ε;
+      ModSem.initial_st := tt↑;
+                                   |}
+    .
+  End SKENV.
+
+  Definition Wrap: Mod.t := {|
+    Mod.get_modsem := fun skenv => WrapSem skenv;
+    Mod.sk := Sk.unit;
+  |}
+  .
+
+End PROOF.
+
+(* Definition cmpspecs: gname -> option (Z -> Z -> Z) := *)
+(*   fun fn => option_map snd (List.find (fun '(str, _) => eqb str fn) [("compare", mycmp)]). *)
